# Arithmetic sequence
Finding **Arithmetic sequence** (difference between consecutive terms is constant plus or minus)

$$
a_n = a_1 + (n-1)d
$$


# Geometric sequence
$$
a_n = ar^{n-1}
$$

# Alternating signs
1, -1, 1, -1, 1, -1

$$
a_n = (-1)^{n+1}
$$

# Compound Interest Geometric sequence Formula:
$$
$P(1+r)^n
$$

# The sum of the first n integers
$$
\sum_{k=1}^{n}k = 1+2+3+....+ n = \frac{n(n+1)}{2}
$$


# The sum of the squares of the first n integers
$$
\begin{align}
\sum_{k=1}^{n}k^2 = 1^2+2^2+3^2+....+ n^2  \\
= \frac{n(n+1)(2n+1)}{6} \\
= \frac{1}{3}n^3 + \frac{1}{2}n^2 + \frac{1}{6}n
\end{align}
$$

# Summation of arithmetic sequence:
$$
S_n=\frac{n(2a+(n-1)d)}{2}
$$
$$
S_n = \frac{n(a_1+a_n)}{2}
$$

# Summation of geometric sequence:
$$
Sn = \frac{a(1-r^n)}{1-r}
$$

$$
Sn = \frac{a(r^n-1)}{r-1}
$$

# Summation of infinite Sequence
$$\frac{a}{1 - r}$$
# Division Theorem:
Let `a` be an integer and `d` a positive number

$$
0 \ge r < d \text{, such that } a = dq+r
$$

# Congruent modulo: Formula:
$$a - b = m(q_1 - q_2)$$

`a` is congruent to `b` modulo `m` if:

$$
a \bmod{m} = b \bmod{m}
$$
Thus,
$$
a \equiv b \bmod{m}
$$
$$
m \mid(a-b)
$$

# Basic modular arithmetic: Theorem 1
$$
a +c \equiv b+d \bmod m
$$

# Basic modular arithmetic: Theorem2:
let m be a positive integer. if `a` congruent `b` mod `m` and `c` congruent `d` mod `m` then:

$$
ac \equiv db \bmod m
$$

# Basic modular arithmetic: Exponentiation rule: 
$$
a^b \bmod m \equiv ((a \bmod m)^b) \bmod m
$$


# Greatest Common Divisor Formula: 
$$
\begin{align}
\gcd(a,b) = p_1^{\min(a_1, b_1)} p_2^{\min(a_1, b_1)}...p_n^{\min(a_n, b_n)}
\end{align}
$$

# Least Common multiple(LCD): Formula: 
$$
\begin{align}
lcm(a,b) = p_1^{\max(a_1, b_1)} p_2^{\max(a_1, b_1)}...p_n^{\max(a_n, b_n)}
\end{align}
$$

# GCD and LCM Formula:
$$
gcd(a,b)×lcm(a,b)=a×b
$$

